feat(environment): Check environment conflicts

Test/Frontend/Collect.lean
@@ -1,45 +1,49 @@
-import Pantograph
+import Pantograph.Frontend
+import Pantograph.Environment
 import Test.Common
 
 open Lean Pantograph Frontend
 
 namespace Pantograph.Test.Frontend.Collect
 
-def runFrontend { α } (source: String) (f : CompilationStep → FrontendM α) (timeout : UInt32 := 0): MetaM (List α) := do
+abbrev Test := Environment → TestT IO Unit
+
+def runFrontend { α } (env : Environment) (source: String) (f : CompilationStep → FrontendM α) (timeout : UInt32 := 0)
+  : IO (List α) := do
   let filename := "<anonymous>"
-  let (context, state) ← do createContextStateFromFile source filename (← getEnv) {}
+  let (context, state) ← do createContextStateFromFile source filename env {}
   let m := mapCompilationSteps f
   let cancelTk? ← match timeout with
     | 0 => pure .none
     | timeout => .some <$> spawnCancelToken timeout
   m.run { cancelTk? } |>.run context |>.run' state
 
-def test_open : TestT MetaM Unit := do
+def test_open : Test := λ env => do
   let sketch := "
 open Nat
 example : ∀ (n : Nat), n + 1 = Nat.succ n := by
   intro
   apply add_one
   "
-  let errors ← runFrontend sketch λ step => step.msgs.mapM (·.toString)
+  let errors ← runFrontend env sketch λ step => step.msgs.mapM (·.toString)
   checkEq "errors" errors [[], []]
 
-
-def collectNewConstants (source: String) : MetaM (List (List Name)) := do
+def collectNewConstants (env : Environment) (source: String) : IO (List (List Name)) := do
   let filename := "<anonymous>"
-  let (context, state) ← do Frontend.createContextStateFromFile source filename (← getEnv) {}
+  let (context, state) ← do Frontend.createContextStateFromFile source filename env {}
   let m := show FrontendM _ from Frontend.mapCompilationSteps λ step => do
     step.newConstants
   let result ← m.run {} |>.run context |>.run' state
   return result.map (·.toList)
 
-def test_collect_one_constant : TestT MetaM Unit := do
+def test_collect_one_constant : Test := λ env => do
   let input := "
 def mystery : Nat := 123
   "
-  let names ← collectNewConstants input
+  let names ← collectNewConstants env input
   checkEq "constants" names [[`mystery]]
-def test_collect_one_theorem : TestT MetaM Unit := do
+
+def test_collect_one_theorem : Test := λ env => do
   let input := "
 theorem mystery [SizeOf α] (as : List α) (i : Fin as.length) : sizeOf (as.get i) < sizeOf as := by
   match as, i with
@@ -49,14 +53,36 @@ theorem mystery [SizeOf α] (as : List α) (i : Fin as.length) : sizeOf (as.get 
     apply Nat.lt_trans ih
     simp_arith
   "
-  let names ← collectNewConstants input
+  let names ← collectNewConstants env input
   checkEq "constants" names [[`mystery]]
-def test_collect_stub : TestT MetaM Unit := do
+
+def test_collect_stub : Test := λ env => do
   let input := "
 theorem mystery [SizeOf α] (as : List α) (i : Fin as.length) : sizeOf (as.get i) < sizeOf as := sorry
   "
-  let names ← collectNewConstants input
+  let names ← collectNewConstants env input
   checkEq "constants" names [[`mystery]]
+
+def checkFileConflicts (env : Environment) (src dst : String) : IO (Except String Environment):= do
+  let srcEnv ← collectOne src
+  let dstEnv ← collectOne dst
+  ExceptT.run $ Environment.checkConflicts env srcEnv dstEnv
+  where
+  collectOne (source : String) : IO Environment := do
+    let filename := "<anonymous>"
+    let (context, state) ← do createContextStateFromFile source filename env {}
+    let m := collectEndEnvironment
+    m.run { } |>.run context |>.run' state
+
+def test_conflict_simple : Test := λ env => do
+  let src := "
+def x : Nat := sorry
+  "
+  let dst := "
+def x : Nat := 123
+  "
+  let result? ← checkFileConflicts env src dst
+  checkTrue "ok" result?.isOk
 
 def suite (env : Environment): List (String × IO LSpec.TestSeq) :=
   let tests := [
@@ -64,5 +90,6 @@ def suite (env : Environment): List (String × IO LSpec.TestSeq) :=
     ("collect_one_constant", test_collect_one_constant),
     ("collect_one_theorem", test_collect_one_theorem),
     ("collect_stub", test_collect_stub),
+    ("conflict simple", test_conflict_simple),
   ]
-  tests.map (fun (name, test) => (name, runMetaMSeq env $ runTest test))
+  tests.map (fun (name, test) => (name, runTest $ test env))
